examples/process/Rot13.v
@@ -14,37 +14,15 @@ Require LanguageInterface.
 Import -(notations) LanguageInterface.
 Require Import Asm.
 Import Memory Values Integers ListNotations.
-Require Import CompCertStrat.
+Require Import CompCertStrat Load.
+Import Load.STRAT.
 Close Scope list.
 Close Scope Z_scope.
 
 (** * §6.3 Modeling loading and the execution environments *)
 
 (** This file contains the verification of the secret and rot13 example using
-    the strategy framework presented in the paper. There is also a legacy
-    version of this example which can be found in `examples/process/*.v` is
-    proved purely using CompCertO structures. The legacy version is not
-    presented in the paper but it shares some common infrastructures.
-
-    Particularly, this file depends on:
-
-    - models/IntStrat.v: the stratgy model used as the verification framework;
-
-    - examples/SecretAsm.v: manual verification of assembly program secret.s,
-      which corresponds to
-
-        π'_secret : L_secret ≤ Asm(secret.s)
-
-      in the paper;
-
-    - examples/Util.v: various auxiliary definitions and lemmas about the
-      CompCertO correctness theorem
-
-    - examples/process/InitMem.v: the construction of the initial memory that is
-      used to invoke the execution of CompCertO semantics
-
-    - examples/process/Load.v: This file has the loader correctness for the
-      legacy version. Most of the lemmas are also useful here
+    the strategy framework presented in the paper.
 
     We made one simplification to the example presented in the paper: we used
     the shorted string "hello" instead of "hello, world!" so that we don't have
@@ -59,15 +37,6 @@ Notation hello_bytes := [ Byte.repr 104; Byte.repr 101; Byte.repr 108; Byte.repr
 Notation uryyb_bytes := [ Byte.repr 117; Byte.repr 114; Byte.repr 121; Byte.repr 121; Byte.repr 98]%list.
 
 (** ** Strategy-level definitions *)
-
-Definition P : esig := {| op := Genv.symtbl; ar _ := Integers.int |}.
-Inductive F_op : Type := F_read : int -> F_op | F_write : list byte -> F_op.
-Definition F : esig :=
-  {|
-    op := F_op;
-    ar m := match m with F_read _ => list byte | F_write _ => Integers.int end;
-  |}.
-Definition S : esig := F + F.
 
 Arguments compose_when {E F G}%esig_scope {i j k} p (σ τ)%strat_scope.
 
@@ -241,715 +210,11 @@ Section STRATEGY.
 
 End STRATEGY.
 
-(** ** C and Asm Loader definitions *)
-
-Require Import CAsm InitMem Maps AST.
-Require Import Conventions Mach Asm.
-Require Import Ctypes.
-Require Import Util.
-
-Lemma rw_sig_size_arguments: size_arguments rw_sig = 0%Z.
-Proof. Transparent Archi.ptr64. cbn. destruct Archi.win64; cbn; lia. Qed.
-
-Section C_LOADER.
-  Import Ctypes Clight.
-  Context (prog: Clight.program).
-  Let sk := AST.erase_program prog.
-
-  (** *** The entry part of the C Loader *)
-  Definition entry_c_play (se: Genv.symtbl) q r i : @play li_c P ready :=
-    @oq li_c P se ::
-    @pq li_c P se (se, q)%embed ::
-    @oa li_c P se (se, q)%embed r ::
-    @pa li_c P se i :: pnil_ready.
-  Inductive valid_entry_c: Genv.symtbl -> c_query -> c_reply -> int -> Prop :=
-  | valid_entry_c_intro se b m main f q r i m'
-    (HM: init_mem se sk = Some m)
-    (HB: Genv.find_symbol se main = Some b)
-    (HMAIN: prog_main prog = Some main)
-    (HF: (prog_defmap prog) ! main = Some (Gfun f))
-    (HQ: q = cq (Vptr b Ptrofs.zero) main_sig []%list m)
-    (HR: r = cr (Vint i) m') :
-    valid_entry_c se q r i.
-  Definition entry_c : li_c ->> P :=
-    sup se, sup q, sup r, sup i, sup (_: valid_entry_c se q r i), down (entry_c_play se q r i).
-
-  (** *** The runtime part of the C Loader *)
-  Definition read_c_play se q n bytes r : @play S li_c ready :=
-    @oq S li_c (se, q)%embed ::
-    @pq S li_c (se, q)%embed (inl (F_read n)) ::
-    @oa S li_c (se, q)%embed (inl (F_read n)) bytes ::
-    @pa S li_c (se, q)%embed r :: pnil_ready.
-  Inductive valid_read_c: Genv.symtbl -> c_query -> int -> list byte -> c_reply -> Prop :=
-  | valid_read_c_intro se q r vf b ofs n m bytes m'
-    (HVF: Genv.find_funct (Clight.globalenv se prog) vf = Some read)
-    (HREAD: Mem.storebytes m b (Ptrofs.unsigned ofs) (map Byte bytes) = Some m')
-    (HLEN: (Z.of_nat (length bytes) <= Int.unsigned n)%Z)
-    (HQ: q = cq vf rw_sig [Vint (Int.repr 0); Vptr b ofs; Vint n]%list m)
-    (HR: r = cr (Vint (Int.repr (Z.of_nat (length bytes)))) m') :
-    valid_read_c se q n bytes r.
-  Definition read_c : S ->> li_c :=
-    sup se, sup q, sup n, sup bytes, sup r, sup (_: valid_read_c se q n bytes r), down (read_c_play se q n bytes r).
-  Definition write_c_play se q bytes n r : @play S li_c ready :=
-    @oq S li_c (se, q)%embed ::
-    @pq S li_c (se, q)%embed (inr (F_write bytes)) ::
-    @oa S li_c (se, q)%embed (inr (F_write bytes)) n ::
-    @pa S li_c (se, q)%embed r :: pnil_ready.
-  Inductive valid_write_c: Genv.symtbl -> c_query -> list byte -> Int.int -> c_reply -> Prop :=
-  | valid_write_c_intro se q r vf b ofs len n m bytes 
-    (HVF: Genv.find_funct (Clight.globalenv se prog) vf = Some write)
-    (HWRITE: Mem.loadbytes m b (Ptrofs.unsigned ofs) len = Some (map Byte bytes))
-    (HI: (0 <= len < Int.modulus - 1)%Z)
-    (HQ: q = cq vf rw_sig [Vint (Int.repr 1); Vptr b ofs; Vint (Int.repr len)]%list m)
-    (HR: r = cr (Vint n) m) :
-    valid_write_c se q bytes n r.
-  Definition write_c : S ->> li_c :=
-    sup se, sup q, sup bytes, sup n, sup r, sup (_: valid_write_c se q bytes n r), down (write_c_play se q bytes n r).
-  Definition runtime_c : S ->> li_c := join read_c write_c.
-  Definition load_c_prog : S ->> P :=
-    entry_c ⊙ (lts_strat (Clight.semantics1 prog)) ⊙ closure runtime_c.
-  Definition load_c_sem (L: Smallstep.semantics li_c li_c) : S ->> P :=
-    entry_c ⊙ (lts_strat L) ⊙ closure runtime_c.
-
-End C_LOADER.
-
-Section ASM_LOADER.
-  Import Asm.
-  Context (prog: Asm.program).
-  Let sk := erase_program prog.
-
-  (** *** The entry part of the Asm Loader *)
-  Definition entry_asm_play (se: Genv.symtbl) q r rv : @play li_asm P ready :=
-    @oq li_asm P se ::
-    @pq li_asm P se (se, q)%embed ::
-    @oa li_asm P se (se, q)%embed r ::
-    @pa li_asm P se rv :: pnil_ready.
-  Inductive valid_entry_asm: Genv.symtbl -> (regset * Mem.mem) -> (regset * Mem.mem) -> int -> Prop :=
-  | valid_entry_asm_intro se rs m rs' m' i vf b f main
-    (HM: init_mem se sk = Some m)
-    (HMAIN: AST.prog_main prog = Some main)
-    (HF: (prog_defmap prog) ! main = Some (Gfun f))
-    (HB: Genv.find_symbol se main = Some b)
-    (HVF: vf = Vptr b Ptrofs.zero)
-    (HRS: rs = (((Pregmap.init Vundef) # PC <- vf) # RSP <- vf) # RA <- Vnullptr)
-    (HRS': rs'#(IR RAX) = Vint i) :
-    valid_entry_asm se (rs, m) (rs', m') i.
-  Definition entry_asm : li_asm ->> P :=
-    sup se, sup q, sup r, sup i, sup (_: valid_entry_asm se q r i), down (entry_asm_play se q r i).
-
-  (** *** The runtime part of the Asm Loader *)
-  Definition read_asm_play se q n bytes r : @play S li_asm ready :=
-    @oq S li_asm (se, q)%embed ::
-    @pq S li_asm (se, q)%embed (inl (F_read n)) ::
-    @oa S li_asm (se, q)%embed (inl (F_read n)) bytes ::
-    @pa S li_asm (se, q)%embed r :: pnil_ready.
-  Inductive valid_read_asm: Genv.symtbl -> (regset * Mem.mem) -> Int.int -> list byte -> (regset * Mem.mem) -> Prop :=
-  | valid_read_asm_intro se (rs: regset) m n bytes rs' m' b ofs
-      (HVF: Genv.find_funct (Genv.globalenv se prog) rs#PC = Some read_asm)
-      (HDI: rs#RDI = Vint (Int.repr 0))
-      (HSI: rs#RSI = Vptr b ofs)
-      (HDX: rs#RDX = Vint n)
-      (HN: (Z.of_nat (length bytes) <= Int.unsigned n)%Z)
-      (HM: Mem.storebytes m b (Ptrofs.unsigned ofs) (map Byte bytes) = Some m')
-      (HAX: rs' = (rs#RAX <- (Vint (Int.repr (Z.of_nat (length bytes)))))#PC <- (rs#RA)) :
-    valid_read_asm se (rs, m) n bytes (rs', m').
-  Definition read_asm : S ->> li_asm :=
-    sup se, sup q, sup n, sup bytes, sup r, sup (_: valid_read_asm se q n bytes r), down (read_asm_play se q n bytes r).
-  Definition write_asm_play se q bytes n r : @play S li_asm ready :=
-    @oq S li_asm (se, q)%embed ::
-    @pq S li_asm (se, q)%embed (inr (F_write bytes)) ::
-    @oa S li_asm (se, q)%embed (inr (F_write bytes)) n ::
-    @pa S li_asm (se, q)%embed r :: pnil_ready.
-  Inductive valid_write_asm: Genv.symtbl -> (regset * Mem.mem) -> list byte -> Int.int -> (regset * Mem.mem) -> Prop :=
-  | valid_write_asm_intro se (rs: regset) m bytes n rs' b ofs r
-      (HVF: Genv.find_funct (Genv.globalenv se prog) rs#PC = Some write_asm)
-      (HDI: rs#RDI = Vint (Int.repr 1))
-      (HSI: rs#RSI = Vptr b ofs)
-      (HDX: rs#RDX = Vint (Int.repr n))
-      (* HI is for determinism *)
-      (HI: (0 <= n < Int.modulus - 1)%Z)
-      (HM: Mem.loadbytes m b (Ptrofs.unsigned ofs) n = Some (map Byte bytes))
-      (HAX: rs' = (rs#RAX <- (Vint r))#PC <- (rs#RA)) :
-    valid_write_asm se (rs, m) bytes r (rs', m).
-  Definition write_asm : S ->> li_asm :=
-    sup se, sup q, sup bytes, sup n, sup r, sup (_: valid_write_asm se q bytes n r), down (write_asm_play se q bytes n r).
-  Definition runtime_asm : S ->> li_asm := join read_asm write_asm.
-  Definition load_asm_prog : S ->> P :=
-    entry_asm ⊙ (lts_strat (Asm.semantics prog)) ⊙ closure runtime_asm.
-  Definition load_asm_sem (L: Smallstep.semantics li_asm li_asm) : S ->> P :=
-    entry_asm ⊙ (lts_strat L) ⊙ closure runtime_asm.
-
-End ASM_LOADER.
-
-Local Hint Constructors pcoh : core.
-
-(** Deterministic property of the asm runtime *)
-
-Instance runtime_asm_determ tp: Deterministic (runtime_asm tp).
-Proof.
-  Ltac dd := dependent destruction Hs; dependent destruction Ht; eauto.
-  Ltac om := match goal with
-    | [ |- pcoh (oq ?x :: _) (oq ?y :: _) ] =>
-        let H := fresh "H" in
-        destruct (classic (x = y)); [ inv H | ]; eauto
-    | [ |- pcoh (oa ?x :: _) (oa ?y :: _) ] =>
-        let H := fresh "H" in
-        destruct (classic (x = y)); [ inv H | ]; eauto
-    end.
-  split. intros s t Hs Ht.
-  unfold runtime_asm in *.
-  destruct Hs as [[|] (?&?&?&?&?&Hs1&Hs)];
-    destruct Ht as [[|] (?&?&?&?&?&Ht1&Ht)]; cbn in *; dd.
-  - om. constructor. dd.
-    assert (x1 = x6) as ->.
-    { inv Hs1. inv Ht1. congruence. }
-    constructor. dd.
-    om. constructor. dd.
-    inv Hs1. inv Ht1.
-    rewrite HSI in HSI0. inv HSI0.
-    rewrite HM in HM0. inv HM0. repeat constructor. dd.
-  - inv Ht1. inv Hs1. eapply pcons_pcoh_oq; eauto.
-    intros A. inv A. rewrite HDI in HDI0. inv HDI0.
-  - inv Ht1. inv Hs1. eapply pcons_pcoh_oq; eauto.
-    intros A. inv A. rewrite HDI in HDI0. inv HDI0.
-  - om. constructor. dd.
-    assert (x1 = x6) as <-.
-    { inv Hs1. inv Ht1. rewrite HSI in HSI0. inv HSI0.
-      rewrite HDX in HDX0.
-      exploit int_repr_inj. apply HI. apply HI0. congruence.
-      intros <-. rewrite HM in HM0.
-      inv HM0. eapply map_inj; eauto.
-      intros. inv H. easy. }
-    constructor. dd.
-    om. constructor. dd. dd.
-    inv Hs1. inv Ht1. repeat constructor.
-Qed.
-
-(** ** Loader correctness *)
-
-Section LOADER_CORRECT.
-  Context p tp (Hp: match_prog p tp).
-
-  Lemma Hsk: erase_program p = erase_program tp.
-  Proof.
-    apply clight2_semantic_preservation in Hp.
-    destruct Hp. destruct X. apply fsim_skel.
-  Qed.
-
-  Transparent Archi.ptr64.
-  Opaque match_prog.
-
-  Lemma entry_correct: rsq CAsm.cc_compcert vid (entry_c p) (entry_asm tp).
-  Proof.
-    intros x (se & q & r & i & H & Hx). inv H. cbn in Hx. rewrite Hx. clear Hx.
-    assert (Hmain: (prog_defmap (erase_program p)) ! main = Some (Gfun tt)).
-    { rewrite erase_program_defmap. unfold option_map. setoid_rewrite HF. reflexivity. }
-    assert (exists tf, (prog_defmap tp) ! main = Some (Gfun tf)) as (tf & Htf).
-    { rewrite Hsk in Hmain. rewrite erase_program_defmap in Hmain.
-      unfold option_map in Hmain.
-      destruct (prog_defmap tp) ! main as [[tf|]|] eqn: Htf; inv Hmain.
-      exists tf. split; eauto. }
-    assert (Htpmain: AST.prog_main tp = Some main).
-    { replace (AST.prog_main tp) with (AST.prog_main (erase_program tp)) by reflexivity.
-      rewrite <- Hsk. apply HMAIN. }
-    unfold entry_c_play. apply rsp_oq. {
-      cbn. eexists se, (_, m), ((Pregmap.init Vundef)#RAX <- (Vint i), m'), i.
-      eexists. econstructor; eauto.
-      - rewrite <- Hsk. eauto.
-      - constructor. }
-    intros q Hq. cbn in Hq. subst q.
-    set (rs :=  (((Pregmap.init Vundef) # PC <- (Vptr b Ptrofs.zero)) # RSP <- (Vptr b Ptrofs.zero)) # RA <- Vnullptr).
-    eapply rsp_pq with (m2 := (se, Datatypes.pair rs m)%embed).
-
-    assert (exists w, LanguageInterface.match_query cc_compcert w
-      {| cq_vf := Vptr b Ptrofs.zero; cq_sg := main_sig; cq_args := []; cq_mem := m |} (rs, m) /\ match_senv cc_compcert w se se).
-    {
-      eexists. split.
-      - unfold cc_compcert.
-        (* cklr *)
-        cbn. instantiate (1 := (se, existT _ 0%nat _, _)).
-        exists (cq (Vptr b Ptrofs.zero) main_sig [] m). split.
-        { reflexivity. }
-        (* inv wt_c *)
-        instantiate (1 := (se, (se, main_sig), _)).
-        exists (cq (Vptr b Ptrofs.zero) main_sig [] m). split.
-        { repeat constructor. }
-        (* lessdef_c *)
-        instantiate (1 := (se, tt, _)).
-        exists (cq (Vptr b Ptrofs.zero) main_sig [] m). split.
-        { repeat constructor. }
-        (* cc_c_asm *)
-        instantiate (1 := (se, caw main_sig
-                    (((Pregmap.init Vundef) # PC
-                      <- (Vptr b Ptrofs.zero)# RSP
-                      <- (Vptr b Ptrofs.zero))# RA
-                     <- Vnullptr) m, _)).
-        eexists ((((Pregmap.init Vundef) # PC
-                   <- (Vptr b Ptrofs.zero)) # RSP
-                  <- (Vptr b Ptrofs.zero)) # RA
-                 <- Vnullptr, m). split.
-        { econstructor; cbn; try constructor; eauto.
-          - destruct Archi.win64; cbn; try easy.
-          - repeat constructor. red. unfold size_arguments.
-            cbn. destruct Archi.win64; reflexivity.
-          - erewrite init_mem_nextblock; eauto.
-            exploit @Genv.genv_symb_range; eauto.
-          - easy.
-          - easy. }
-        (* cc_asm vainj *)
-        instantiate (1 := (se, Inject.injw (Mem.flat_inj (Mem.nextblock m)) (Mem.nextblock m) (Mem.nextblock m))).
-        repeat apply conj; cbn; eauto; try easy.
-        + intros.
-          assert (Val.inject (Mem.flat_inj (Mem.nextblock m)) (Vptr b Ptrofs.zero) (Vptr b Ptrofs.zero)).
-          { eapply Val.inject_ptr. unfold Mem.flat_inj.
-             destruct plt. reflexivity.
-             exfalso. apply n. erewrite init_mem_nextblock; eauto.
-             eapply Genv.genv_symb_range; eauto.
-             reflexivity. }
-          destruct r; eauto; cbn; try constructor; eauto.
-          destruct i0; eauto; cbn.
-        + constructor; cbn.
-          * erewrite init_mem_nextblock; eauto. reflexivity.
-          * eapply InitMem.init_mem_romatch. eauto.
-          * constructor. eapply initmem_inject; eauto.
-      - cbn. repeat apply conj; eauto. constructor. eauto.
-        constructor; cbn; erewrite init_mem_nextblock; eauto; try easy.
-        apply Load.match_stbls_flat_inj.
-    }
-
-    destruct H as (w & Hq & Hse).  econstructor; eauto.
-    eapply rsp_oa. {
-      cbn. eexists se, (_, m), ((Pregmap.init Vundef)#RAX <- (Vint i), m'), i.
-      eexists. econstructor; eauto.
-      - rewrite <- Hsk. eauto.
-      - repeat constructor. }
-    intros [rs1 m1] Hr. eapply rcp_forbid_mr in Hr; eauto.
-    3: {
-      unfold cc_compcert.
-      (* cklr *)
-      cbn. instantiate (1 := (se, existT _ 0%nat _, _)).
-      exists (cq (Vptr b Ptrofs.zero) main_sig [] m). split.
-      { reflexivity. }
-      (* inv wt_c *)
-      instantiate (1 := (se, (se, main_sig), _)).
-      exists (cq (Vptr b Ptrofs.zero) main_sig [] m). split.
-      { repeat constructor. }
-      (* lessdef_c *)
-      instantiate (1 := (se, tt, _)).
-      exists (cq (Vptr b Ptrofs.zero) main_sig [] m). split.
-      { repeat constructor. }
-      (* cc_c_asm *)
-      instantiate (1 := (se, caw main_sig
-                               (((Pregmap.init Vundef) # PC
-                                 <- (Vptr b Ptrofs.zero)# RSP
-                                 <- (Vptr b Ptrofs.zero))# RA
-                                <- Vnullptr) m, _)).
-      eexists ((((Pregmap.init Vundef) # PC
-                 <- (Vptr b Ptrofs.zero)) # RSP
-                <- (Vptr b Ptrofs.zero)) # RA
-               <- Vnullptr, m). split.
-      { econstructor; cbn; try constructor; eauto.
-        - destruct Archi.win64; cbn; try easy.
-        - repeat constructor. red. unfold size_arguments.
-          cbn. destruct Archi.win64; reflexivity.
-        - erewrite init_mem_nextblock; eauto.
-          exploit @Genv.genv_symb_range; eauto.
-        - easy.
-        - easy. }
-      (* cc_asm vainj *)
-      instantiate (1 := (se, Inject.injw (Mem.flat_inj (Mem.nextblock m)) (Mem.nextblock m) (Mem.nextblock m))).
-      repeat apply conj; cbn; eauto; try easy.
-      + intros.
-        assert (Val.inject (Mem.flat_inj (Mem.nextblock m)) (Vptr b Ptrofs.zero) (Vptr b Ptrofs.zero)).
-        { eapply Val.inject_ptr. unfold Mem.flat_inj.
-          destruct plt. reflexivity.
-          exfalso. apply n. erewrite init_mem_nextblock; eauto.
-          eapply Genv.genv_symb_range; eauto.
-          reflexivity. }
-        destruct r; eauto; cbn; try constructor; eauto.
-        destruct i0; eauto; cbn.
-      + constructor; cbn.
-        * erewrite init_mem_nextblock; eauto. reflexivity.
-        * eapply InitMem.init_mem_romatch. eauto.
-        * constructor. eapply initmem_inject; eauto.
-    }
-    2: {
-      cbn. repeat apply conj; eauto. constructor. eauto.
-      constructor; cbn; erewrite init_mem_nextblock; eauto; try easy.
-      apply Load.match_stbls_flat_inj.
-    }
-    cbn in Hr. destruct Hr as (r3 & Hr3 & HR). inv Hr3.
-    destruct HR as (r3 & Hr3 & HR). inv Hr3.
-    destruct HR as (r3 & Hr3 & HR). inv Hr3. inv H3.
-    destruct HR as (r3 & Hr3 & HR). inv Hr3. cbn in *.
-    destruct HR as ((? & ?) & ? & Hr). 
-    inv Hr. specialize (H1 RAX). rewrite <- H5 in H1.
-    cbn in H1. inv H1.
-
-    eapply rsp_pa with (r2 := i).
-    { intros Hx. inv Hx. apply H3. apply JMeq_refl. }
-    apply rsp_ready. cbn. eexists _, (rs, _), (rs1, _), _. eexists.
-    { econstructor; eauto.
-      * rewrite <- Hsk. eauto.
-      * subst rs. cbn. rewrite H12. easy. }
-    unfold entry_asm_play. reflexivity.
-    Unshelve. all: cbn; exact tt.
-  Qed.
-
-  Import Compiler CKLR VAInject Inject.
-  Import -(notations) CallconvAlgebra.
-  Definition inj_state := (block * ptrofs * Mem.mem)%type.
-  Inductive match_inj_state:
-    ccworld (cc_star cc_cklrs) -> world vainj -> cc_ca_world -> inj_state -> inj_state -> Prop :=
-  | match_inj_state_intro wn wi b1 ofs1 m1 b2 ofs2 m2 caw se 
-      (HM: Load.mm_ca wn (se, wi) (caw_m caw) m1 m2) (HP: Load.mp_ca wn wi b1 ofs1 b2 ofs2):
-      match_inj_state wn (se, wi) caw (b1, ofs1, m1) (b2, ofs2, m2).
-
-  Lemma runtime_correct: rsq vid CAsm.cc_compcert (runtime_c p) (runtime_asm tp).
-  Proof.
-    setoid_rewrite cc_conv_expand. apply rsq_sup. apply runtime_asm_determ.
-    { constructor. apply None. }
-    intros [w|].
-    2: { intros s ([|] & Hs).
-         - destruct Hs as (se & q & n & bs & r & H & Hs). rewrite Hs. clear Hs.
-           unfold read_c_play. apply rsp_oq. {
-             exists true. cbn. inv H. eexists se, (((((Pregmap.init Vundef)#PC <- vf)#RDI <- (Vint (Int.repr 0))#RSI <- (Vptr b ofs))#RDX <- (Vint n)), m), n, bs, (_, m').
-             eexists. 2: constructor.
-             econstructor; cbn; eauto.
-             eapply match_prog_read. 4: eauto.
-             apply Hp.
-             apply Genv.match_stbls_id.
-             apply val_inject_refl. }
-           intros q2 Hq2. xinv Hq2.
-         - destruct Hs as (se & q & bs & n & r & H & Hs). rewrite Hs. clear Hs.
-           unfold write_c_play. apply rsp_oq. {
-             exists false. cbn. inv H. eexists se, (((((Pregmap.init Vundef)#PC <- vf)#RDI <- (Vint (Int.repr 1))#RSI <- (Vptr b ofs))#RDX <- (Vint (Int.repr len))), m), bs, n, (_, m).
-             eexists. 2: constructor.
-             econstructor; cbn; eauto.
-             eapply match_prog_write. 4: eauto.
-             apply Hp.
-             apply Genv.match_stbls_id.
-             apply val_inject_refl. }
-           intros q2 Hq2. xinv Hq2. }
-    intros s (i & Hs). destruct i; cbn in Hs.
-    Ltac inv_lessdef:=
-      match goal with
-      | [ H: Val.lessdef_list _ _ |- _ ] => inv H
-      | [ H: Val.lessdef _ _ |- _ ] => inv H
-      end.
-    - destruct Hs as (se & q & n & bs & r & H & Hs). rewrite Hs. clear Hs.
-      inv H. unfold read_c_play. apply rsp_oq. {
-        exists true. cbn. eexists se, (((((Pregmap.init Vundef)#PC <- vf)#RDI <- (Vint (Int.repr 0))#RSI <- (Vptr b ofs))#RDX <- (Vint n)), m), n, bs, (_, m').
-        eexists. 2: constructor.
-        econstructor; cbn; eauto.
-        eapply match_prog_read. 4: eauto.
-        apply Hp.
-        apply Genv.match_stbls_id.
-        apply val_inject_refl. }
-      intros q Hq. cbn in Hq. dependent destruction Hq.
-      eapply rsp_pq with (m2 := inl (F_read n)). reflexivity.
-      eapply rsp_oa. {
-        exists true. cbn. 
-      set (w1 := (Load.nw_of_world w)). set (w2 := (Load.injw_of_world w)). set (w3 := (Load.caw_of_world w)).
-      unfold CAsm.cc_compcert in *. cbn in w, HM |- *.
-      eprod_crush. destruct s7.
-      match goal with
-      | [ H: Invariant.rel_inv _ _ _ |- _ ] => inv H; eprod_crush; subst
-      end.
-      (* cklrs *)
-      eapply (Load.cklrs_match_query_inv' (existT _ x2 c0)) in H as
-          (mx & bx & ofsx & vfx & Hqx & Hmx & Hpx & Hvx). subst x0. cbn in *.
-      (* lessdef *)
-      inv H1. repeat inv_lessdef.
-      (* cc_c_asm: need to show args_removed changes nothing *)
-      inv H2. inv HRM. inv H.
-      2: { match goal with
-          | [ H: size_arguments _ > 0 |- _ ] => rewrite rw_sig_size_arguments in H  end.
-           lia. }
-      (* cc_asm vainj *)
-      destruct m2. destruct H3 as (Hreg & Hpc & Him).
-      (* arguments *)
-      match goal with
-      | [ H: cons _ _ = _ |- _ ] => cbn in H; rewrite Hwin in H; cbn in H; inv H
-      end.
-
-      assert (exists b' ofs', r0#RSI = Vptr b' ofs' /\ Val.inject i (Vptr bx ofsx) (Vptr b' ofs')) as (b' & ofs' & Hofs & Hb').
-      { specialize (Hreg RSI). rewrite <- H2 in Hreg. inv Hreg.
-        eexists _, _. split; eauto. }
-
-      assert (HMS: match_inj_state w1 w2 w3 (b, ofs, m) (b', ofs', m0)).
-      { econstructor.
-        (* mem *)
-        - inv Him. econstructor; eauto. reflexivity.
-          cbn. apply Mem.unchanged_on_refl.
-        (* ptr *)
-        - econstructor; eauto. inv Hb'. constructor; eauto. }
-      inv HMS.
-      exploit Load.ca_storebytes; eauto. intros (mx1 & Hs & Hm).
-      inv Hm.
-
-        eexists _, _, _, _, (_, _).
-        eexists.
-        2: { unfold read_asm_play. repeat constructor. }
-        econstructor; eauto.
-      + cbn in HVF. cbn in HSE.  eprod_crush. inv H8.
-        eapply ca_find_funct_read; eauto.
-        apply H7. apply HVF.
-      + specialize (Hreg RDI). rewrite <- H0 in Hreg. inv Hreg; eauto.
-      + specialize (Hreg RDX). rewrite <- H3 in Hreg. inv Hreg; eauto.
-      }
-      intros r2 H2. cbn in H2. apply not_and_or in H2 as [H2|H2]. easy.
-      assert (bs = r2) as <-.
-      { apply NNPP. intros Hx. apply H2. intros Hy. apply Hx.
-        apply JMeq_eq; eauto. } clear H2.
-
-      set (w1 := (Load.nw_of_world w)). set (w2 := (Load.injw_of_world w)). set (w3 := (Load.caw_of_world w)).
-      unfold CAsm.cc_compcert in *. cbn in w, HM |- *.
-      eprod_crush. destruct s7.
-      match goal with
-      | [ H: Invariant.rel_inv _ _ _ |- _ ] => inv H; eprod_crush; subst
-      end.
-      (* cklrs *)
-      eapply (Load.cklrs_match_query_inv' (existT _ x2 c0)) in H as
-          (mx & bx & ofsx & vfx & Hqx & Hmx & Hpx & Hvx). subst x0. cbn in *.
-      (* lessdef *)
-      inv H1. repeat inv_lessdef.
-      (* cc_c_asm: need to show args_removed changes nothing *)
-      inv H2. inv HRM. inv H.
-      2: { match goal with
-          | [ H: size_arguments _ > 0 |- _ ] => rewrite rw_sig_size_arguments in H  end.
-           lia. }
-      (* cc_asm vainj *)
-      destruct m2. destruct H3 as (Hreg & Hpc & Him).
-      (* arguments *)
-      match goal with
-      | [ H: cons _ _ = _ |- _ ] => cbn in H; rewrite Hwin in H; cbn in H; inv H
-      end.
-
-      assert (exists b' ofs', r0#RSI = Vptr b' ofs' /\ Val.inject i (Vptr bx ofsx) (Vptr b' ofs')) as (b' & ofs' & Hofs & Hb').
-      { specialize (Hreg RSI). rewrite <- H2 in Hreg. inv Hreg.
-        eexists _, _. split; eauto. }
-
-      assert (HMS: match_inj_state w1 w2 w3 (b, ofs, m) (b', ofs', m0)).
-      { econstructor.
-        (* mem *)
-        - inv Him. econstructor; eauto. reflexivity.
-          cbn. apply Mem.unchanged_on_refl.
-        (* ptr *)
-        - econstructor; eauto. inv Hb'. constructor; eauto. }
-      inv HMS.
-      exploit Load.ca_storebytes; eauto. intros (mx1 & Hs & Hm).
-      inv Hm.
-      set (v := (Vint (Int.repr (Z.of_nat (length bs))))).
-      eapply rsp_pa with (r2 := ((r0#RAX <- v)#PC <- (r0#RA), mx1)).
-      {
-        intros HR. cbn in HR. dependent destruction HR. apply HN0. clear HM0 HN0.
-
-        (* m --store--> m'
-           |            |
-           |          mm_cklr
-           |            |
-         mm_ca          m2
-           |            |
-           |           inj
-           |            |
-          m0 --store--> mx1
-         *)
-
-        eexists (cr v m2). split.
-        { eapply Load.cklrs_match_reply_intro; eauto. }
-        eexists (cr v m2). split.
-        (* need sig *)
-        { constructor. easy. }
-        eexists (cr v m2). split.
-        { constructor. constructor. }
-        exists ((r#RAX <- v)#PC <- (r#RA), m2). split.
-        { cbn in Hreg |- *.
-          (* destruct w3; cbn in HSG, HRS |- *. *)
-          (* subst caw_sg.  *)
-          constructor; eauto.
-          - intros r1. destruct r1; cbn; eauto. easy.
-          - apply Mem.unchanged_on_refl.
-          - rewrite rw_sig_size_arguments.
-            replace (loc_init_args 0 (r RSP))
-              with (fun (_: block) (_: Z) => False); eauto.
-            repeat (apply Axioms.functional_extensionality; intros).
-            apply PropExtensionality.propositional_extensionality.
-            split; try easy. intros HX. inv HX. lia.
-          - rewrite rw_sig_size_arguments.
-            intros * HX. inv HX. lia. }
-        { exists (s0, wj). split. split; eauto. split.
-          - intros. cbn in Hreg. apply (mi_acc inj) in HJ.
-            destruct r1; cbn; eauto. 
-            destruct i0; cbn; eauto.
-            subst v. eauto.
-          - constructor; eauto. }
-      }
-
-      apply rsp_ready. exists true.
-      eexists _, (r0, m0), _, _, ((r0#RAX <- v)#PC <- (r0#RA), mx1).
-      eexists.
-      { econstructor; eauto.
-      + cbn in HVF. cbn in HSE.  eprod_crush. inv r1.
-        eapply ca_find_funct_read; eauto.
-        apply m1. apply HVF.
-      + specialize (Hreg RDI). rewrite <- H0 in Hreg. inv Hreg; eauto.
-      + specialize (Hreg RDX). rewrite <- H3 in Hreg. inv Hreg; eauto.
-      }
-      cbn. reflexivity.
-    - destruct Hs as (se & q & bs & n & r & H & Hs). rewrite Hs. clear Hs.
-      inv H. unfold write_c_play. apply rsp_oq. {
-        exists false. cbn. eexists se, (((((Pregmap.init Vundef)#PC <- vf)#RDI <- (Vint (Int.repr 1))#RSI <- (Vptr b ofs))#RDX <- (Vint (Int.repr len))), m), bs, n, (_, m).
-        eexists. 2: constructor.
-        econstructor; cbn; eauto.
-        eapply match_prog_write. 4: eauto.
-        apply Hp.
-        apply Genv.match_stbls_id.
-        apply val_inject_refl.
-      }
-      intros q Hq. cbn in Hq. dependent destruction Hq.
-      eapply rsp_pq with (m2 := inr (F_write bs)). reflexivity.
-      eapply rsp_oa. {
-        exists false. cbn.
-
-      set (w1 := (Load.nw_of_world w)). set (w2 := (Load.injw_of_world w)). set (w3 := (Load.caw_of_world w)).
-      destruct m2 as [rs mt].
-      unfold CAsm.cc_compcert in *. cbn in w, HM |- *.
-      destruct HI as [HI1 HI2].
-      eprod_crush. destruct s7.
-      match goal with
-      | [ H: Invariant.rel_inv _ _ _ |- _ ] => inv H; eprod_crush; subst
-      end.
-      eapply (Load.cklrs_match_query_inv' (existT _ x2 c0)) in H as
-          (mx & bx & ofsx & vfx & Hqx & Hmx & Hpx & Hvx). subst x0. cbn in *.
-      (* lessdef *)
-      inv H1. repeat inv_lessdef.
-      (* cc_c_asm: need to show args_removed changes nothing *)
-      inv H2. inv HRM. inv H.
-      2: { match goal with
-        | [ H: size_arguments _ > 0 |- _ ] =>
-            rewrite rw_sig_size_arguments in H; try lia  end. }
-      (* cc_asm vainj *)
-      destruct H3 as (Hreg & Hpc & Him).
-      (* arguments *)
-      match goal with
-      | [ H: cons _ _ = _ |- _ ] => cbn in H; rewrite Hwin in H; cbn in H; inv H
-      end.
-      assert (exists b' ofs', rs#RSI = Vptr b' ofs' /\ Val.inject i (Vptr bx ofsx) (Vptr b' ofs')) as (b' & ofs' & Hofs & Hb').
-      { specialize (Hreg RSI). rewrite <- H2 in Hreg. inv Hreg.
-        eexists _, _. split; eauto. }
-      assert (HCA: Load.mm_ca w1 w2 (caw_m w3) m mt).
-      { inv Him. econstructor; eauto. reflexivity.
-        apply Mem.unchanged_on_refl. }
-
-        eexists _, _, _, _, (_, _).
-        exists. 2: { repeat constructor. }
-         econstructor; cbn; eauto.
-        + cbn in HVF. cbn in HSE.  eprod_crush. inv H8.
-          eapply ca_find_funct_write; eauto.
-          apply H7. apply HVF.
-        + specialize (Hreg RDI). rewrite <- H0 in Hreg. inv Hreg; eauto.
-        + specialize (Hreg RDX). rewrite <- H3 in Hreg. inv Hreg; eauto.
-        + inv Him. eapply Load.ca_loadbytes; eauto.
-          econstructor; eauto. inv Hb'. constructor; eauto.
-      }
-      intros r2 H2. cbn in H2. apply not_and_or in H2 as [H2|H2]. easy.
-      assert (n = r2) as <-.
-      { apply NNPP. intros Hx. apply H2. intros Hy. apply Hx.
-        apply JMeq_eq; eauto. } clear H2.
-      set (w1 := (Load.nw_of_world w)). set (w2 := (Load.injw_of_world w)). set (w3 := (Load.caw_of_world w)).
-      destruct m2 as [rs mt].
-      unfold CAsm.cc_compcert in *. cbn in w, HM |- *.
-      destruct HI as [HI1 HI2].
-      eprod_crush. destruct s7.
-      match goal with
-      | [ H: Invariant.rel_inv _ _ _ |- _ ] => inv H; eprod_crush; subst
-      end.
-      eapply (Load.cklrs_match_query_inv' (existT _ x2 c0)) in H as
-          (mx & bx & ofsx & vfx & Hqx & Hmx & Hpx & Hvx). subst x0. cbn in *.
-      (* lessdef *)
-      inv H1. repeat inv_lessdef.
-      (* cc_c_asm: need to show args_removed changes nothing *)
-      inv H2. inv HRM. inv H.
-      2: { match goal with
-        | [ H: size_arguments _ > 0 |- _ ] =>
-            rewrite rw_sig_size_arguments in H; try lia  end. }
-      (* cc_asm vainj *)
-      destruct H3 as (Hreg & Hpc & Him).
-      (* arguments *)
-      match goal with
-      | [ H: cons _ _ = _ |- _ ] => cbn in H; rewrite Hwin in H; cbn in H; inv H
-      end.
-      assert (exists b' ofs', rs#RSI = Vptr b' ofs' /\ Val.inject i (Vptr bx ofsx) (Vptr b' ofs')) as (b' & ofs' & Hofs & Hb').
-      { specialize (Hreg RSI). rewrite <- H2 in Hreg. inv Hreg.
-        eexists _, _. split; eauto. }
-      
-      set (v := (Vint n)).
-      eapply rsp_pa with (r2 := ((rs#RAX <- v)#PC <- (rs#RA), mt)).
-      {
-        intros HR. cbn in HR. dependent destruction HR. apply HN. clear HM HN.
-        eexists (cr v mx). split.
-        { eapply Load.cklrs_match_reply_intro; eauto. }
-        eexists (cr v mx). split.
-        (* need sig *)
-        { constructor. easy. }
-        eexists (cr v mx). split.
-        { constructor. constructor. }
-        exists ((r#RAX <- v)#PC <- (r#RA), mx). split.
-        { cbn in Hreg |- *. constructor; eauto.
-          - intros r1. destruct r1; cbn; eauto. easy.
-          - apply Mem.unchanged_on_refl.
-          - apply Mem.unchanged_on_refl.
-          - rewrite rw_sig_size_arguments.
-            intros * HX. inv HX. lia. }
-        { exists (s0, i). split. reflexivity. split; eauto.
-          intros. cbn in Hreg. destruct r0; cbn; eauto. destruct i0; cbn; eauto.
-          subst v. eauto. }
-      }
-
-      assert (HCA: Load.mm_ca w1 w2 (caw_m w3) m mt).
-      { inv Him. econstructor; eauto. reflexivity.
-        apply Mem.unchanged_on_refl. }
-
-      apply rsp_ready. exists false.
-      eexists _, (rs, mt), _, _, ((rs#RAX <- v)#PC <- (rs#RA), mt).
-      eexists.
-      { econstructor; eauto.
-        + cbn in HVF. cbn in HSE.  eprod_crush. inv r0.
-          eapply ca_find_funct_write; eauto.
-          apply m0. apply HVF.
-        + specialize (Hreg RDI). rewrite <- H0 in Hreg. inv Hreg; eauto.
-        + specialize (Hreg RDX). rewrite <- H3 in Hreg. inv Hreg; eauto.
-        + inv Him. eapply Load.ca_loadbytes; eauto.
-          econstructor; eauto. inv Hb'. constructor; eauto.
-        + cbn. reflexivity. }
-      cbn. reflexivity.
-      Unshelve. exact (Int.repr 0).
-  Qed.
-
-  Lemma load_sem_correct L_c L_asm:
-    determinate L_asm ->
-    forward_simulation CAsm.cc_compcert CAsm.cc_compcert L_c L_asm ->
-    load_c_sem p L_c [= load_asm_sem tp L_asm.
-  Proof.
-    intros HD HL. eapply rsq_id_conv with (p := rs_ready).
-    eapply rsq_comp_when. constructor. apply entry_correct.
-    eapply rsq_comp_when. constructor.
-    2: { apply rsq_closure. 3: apply runtime_correct.
-         1-2: eauto with typeclass_instances. }
-    apply fsim_rsq; eauto.
-  Qed.
-
-  (* Lemma load_prog_correct : *)
-  (*   load_c_prog p [= load_asm_prog tp. *)
-  (* Abort. *)
-End LOADER_CORRECT.
-
 (** ** Code Proof for the Clight programs *)
 
 (** *** Clight Program rot13.c *)
 
-Require Import Clight Ctypes Cop.
+Require Import AST Clight Ctypes Cop Maps.
 
 Definition secret_c_main_id: positive := 1.
 Definition secret_c_rot13_id: positive := 2.
@@ -1046,6 +311,7 @@ Program Definition sr_clight: Clight.program :=
 Next Obligation. reflexivity. Qed.
 
 Require SecretAsm.
+Require Import InitMem Util.
 
 (** *** Correctness proof of the secret program *)
 
@@ -1564,7 +830,7 @@ Section DECODE.
     assert (Hflag: Mem.alloc_flag m = true).
     { eapply init_mem_alloc_flag; eauto. }
     edestruct (@Mem.alloc_succeed m 0 100); eauto. destruct x as (m1 & bb1).
-    assert (exists m2, Mem.storebytes m1 bb1 0 (Byte ## uryyb_bytes) = Some m2) as (m2 & Hm2).
+    assert (exists m2, Mem.storebytes m1 bb1 0 (map Byte uryyb_bytes) = Some m2) as (m2 & Hm2).
     { edestruct Mem.range_perm_storebytes. 2: eexists; eauto.
       intros f Hf. cbn in Hf.
       eapply Mem.perm_alloc_2 in e. eauto with mem. lia. }
@@ -1718,7 +984,10 @@ Section DECODE.
     econstructor 4. (* decode.c internal step *)
     { apply star_one. econstructor 1. unfold rw_type. crush_step; eauto; try reflexivity.
       - crush_expr.
-      - crush_expr. eapply eval_Ecast. crush_expr. all: reflexivity. }
+      - crush_expr.
+        constructor. reflexivity.
+        eapply eval_Ecast. crush_expr. reflexivity.
+        constructor. reflexivity. }
     econstructor 2. (* decode.c calls read *)
     { repeat econstructor. apply Hb8'. intros [|] Hj.
       - unfold valid_query in Hj. cbn in Hj.
@@ -1755,7 +1024,7 @@ Section DECODE.
     econstructor 4. (* decode.c internal step *)
     { apply star_one. econstructor 1. crush_step. 4: apply Hb4'. 1,4: reflexivity.
       - crush_expr. constructor. reflexivity.
-      - crush_expr. }
+      - crush_expr. constructor. reflexivity. }
     econstructor 4. (* decode.c calls rot13.c *)
     { apply star_one. econstructor 2.
       - econstructor; eauto.
@@ -1827,7 +1096,9 @@ Section DECODE.
     { apply star_one. econstructor 3; constructor. }
     do 3 one_trivial_step.
     econstructor 4. (* decode.c calls write *)
-    { apply star_one. econstructor 1. crush_step; crush_expr. }
+    { apply star_one. econstructor 1. crush_step; crush_expr.
+      constructor. reflexivity.
+      constructor. reflexivity. }
     econstructor 2. (* decode.c calls write *)
     { repeat econstructor. apply Hb6'.
       intros [|] Hj.
@@ -1860,7 +1131,8 @@ Section DECODE.
     econstructor 4. (* decode.c internal step *)
     { apply star_one. econstructor 1. crush_step. }
     econstructor 4. (* decode.c internal step *)
-    { apply star_one. econstructor 1. crush_step; crush_expr. }
+    { apply star_one. econstructor 1. crush_step; crush_expr.
+      constructor. reflexivity. }
     econstructor 3.
     { repeat econstructor. }
   Qed.
